{
  "@context": {
    "rdfs": "http://www.w3.org/2000/01/rdf-schema#",
    "schema": "http://schema.org/",
    "re": "https://mangrove.reviews/schema"
  },
  "@graph": [
    {
      "@id": "re:experienceContext",
      "@type": "rdfs:Property",
      "rdfs:comment": "Context in which the reviewer primarily had experience with the subject.",
      "rdfs:label": "experienceContext",
      "schema:domainIncludes": "Review",
      "schema:rangeIncludes": "ExperienceContext"
    },
    {
      "@id": "re:ExperienceContext",
      "@type": "rdfs:Class",
      "rdfs:comment": "An enumeration class that lists common contexts in which the reviewer primarily had experience with the subject.",
      "rdfs:label": "Review",
      "rdfs:subClassOf": "schema:Text"
    },
    {
      "@id": "re:reviewerIndex",
      "@type": "rdfs:Property",
      "rdfs:comment": "Unique index used by the reviewer, usually indicating a ranking in a list.",
      "rdfs:label": "reviewerIndex",
      "schema:domainIncludes": "Review",
      "schema:rangeIncludes": "schema:Integer"
    },
    {
      "@id": "re:isGenerated",
      "@type": "rdfs:Property",
      "rdfs:comment": "True if the review has been left by a review generating bot.",
      "rdfs:label": "isGenerated",
      "schema:domainIncludes": "Review",
      "schema:rangeIncludes": "schema:Boolean"
    },
    {
      "@id": "re:isAffiliated",
      "@type": "rdfs:Property",
      "rdfs:comment": "True if the review has been left by a reviewer affiliated with the subject, such as business owner or employee.",
      "rdfs:label": "isAffiliated",
      "schema:domainIncludes": "Review",
      "schema:rangeIncludes": "schema:Boolean"
    },
    {
      "@id": "re:isPersonalExperience",
      "@type": "rdfs:Property",
      "rdfs:comment": "True if if the review has been left by a reviewer who had direct experience with the subject of the review and is not based on a third party account.",
      "rdfs:label": "isPersonalExperience",
      "schema:domainIncludes": "Review",
      "schema:rangeIncludes": "schema:Boolean"
    }
  ]
}